proof/invariant-abstract/RISCV64/ArchDetSchedAux_AI.thy
@@ -274,6 +274,14 @@ lemma perform_asid_control_invocation_pred_map_sc_refill_cfgs_of:
   by (wpsimp wp: delete_objects_pred_map_sc_refill_cfgs_of
            comb: hoare_drop_imp)
 
+lemma perform_asid_control_invocation_inactive_implies_zero_budget:
+  "perform_asid_control_invocation aci
+   \<lbrace>\<lambda>s. pred_map inactive_scrc (sc_refill_cfgs_of s) p
+        \<longrightarrow> pred_map (\<lambda>cfg. scrc_budget cfg = 0) (sc_refill_cfgs_of s) p\<rbrace>"
+  unfolding perform_asid_control_invocation_def
+  by (wpsimp wp: delete_objects_pred_map_sc_refill_cfgs_of
+           comb: hoare_drop_imp)
+
 crunches perform_asid_control_invocation
   for valid_machine_time[wp]: "valid_machine_time"
   and cur_sc[wp]: "\<lambda>s. P (cur_sc s)"
@@ -295,6 +303,7 @@ lemma perform_asid_control_invocation_valid_sched:
                                    perform_asid_control_invocation_sc_at_pred_n
                                    perform_asid_control_invocation_valid_idle
                                    perform_asid_control_invocation_pred_map_sc_refill_cfgs_of
+                                   perform_asid_control_invocation_inactive_implies_zero_budget
                                    hoare_vcg_all_lift
                              simp: ipc_queued_thread_state_live live_sc_def)+
   done
